RelationalAlgebra/Equivalence/Equivalence.lean
@@ -83,20 +83,20 @@ variable {ρ α μ : Type} [Inhabited α] [Inhabited ρ] [LinearOrder α] [Linea
   (brs : Finset α)
 
 /-- Query evaluation equivalence for `RelationInstance` -/
-theorem fol_to_ra_eval (brs_disj : folQ.schema ∩ brs = ∅) (brs_depth : 0 + FOL.depth (toPrenex folQ) < brs.card) (brs_def : default ∉ brs)
+theorem queryToRA_eval (brs_disj : folQ.schema ∩ brs = ∅) (brs_depth : 0 + FOL.depth (toPrenex folQ) < brs.card) (brs_def : default ∉ brs)
   (hμ : ∀v, v ∈ dbi.domain) (hdisj : FOL.disjointSchema brs (folQ.toFormula)) (hdef : default ∉ folQ.schema) :
-    (fol_to_ra_query folQ brs).evaluate dbi (fol_to_ra_query.isWellTyped_def folQ brs_disj brs_depth) = folQ.evaluateAdom dbi := by
+    (queryToRA folQ brs).evaluate dbi (queryToRA.isWellTyped_def folQ brs_disj brs_depth) = folQ.evaluateAdom dbi := by
       simp only [RA.Query.evaluate, FOL.Query.evaluateAdom, RelationInstance.mk.injEq]
       apply And.intro
-      · exact fol_to_ra_query.schema_def folQ
-      · exact fol_to_ra_query.evalT_def folQ hμ hdisj hdef brs_disj brs_depth brs_def
+      · exact queryToRA.schema_def folQ
+      · exact queryToRA.evalT_def folQ hμ hdisj hdef brs_disj brs_depth brs_def
 
 /-- Query expressivity equivalence -/
-theorem fol_to_ra (brs : Finset α) (brs_disj : folQ.schema ∩ brs = ∅) (brs_depth : 0 + FOL.depth (toPrenex folQ) < brs.card) (brs_def : default ∉ brs)
+theorem fol_to_ra_equivalence (brs : Finset α) (brs_disj : folQ.schema ∩ brs = ∅) (brs_depth : 0 + FOL.depth (toPrenex folQ) < brs.card) (brs_def : default ∉ brs)
   (hμ : ∀v, v ∈ dbi.domain) (hdisj : FOL.disjointSchema brs (folQ.toFormula)) (hdef : default ∉ folQ.schema) :
     ∃raQ : RA.Query _ _, ∃(h' : raQ.isWellTyped dbi.schema), raQ.evaluate dbi h' = folQ.evaluateAdom dbi := by
-      use fol_to_ra_query folQ brs
-      use fol_to_ra_query.isWellTyped_def folQ brs_disj brs_depth
-      exact fol_to_ra_eval folQ brs brs_disj brs_depth brs_def hμ hdisj hdef
+      use queryToRA folQ brs
+      use queryToRA.isWellTyped_def folQ brs_disj brs_depth
+      exact queryToRA_eval folQ brs brs_disj brs_depth brs_def hμ hdisj hdef
 
 end FOLtoRA
